---
html:
    toc: true
print_background: true
---
<!-- @import "[TOC]" {cmd="toc" depthFrom=1 depthTo=6 orderedList=false} -->

<!-- code_chunk_output -->

- [headline](#headline)
- [Introduction of $\beta$](#introduction-of-beta)

<!-- /code_chunk_output -->

## headline
$$ V_g = \frac{1}{\frac{1}{V_g(0)-V_s-V_{th}}-\frac{K}{C}\tau}+V_{th}+V_{s}$$
$$ V_{gs}=\frac{1}{\frac{1}{V_g(0)-V_s-V_{th}}-\frac{K}{C}\tau}+V_{th}+V_{s}-V_{dd}$$
$$ i_{ds} = \frac{1}{2}k(V_{gs}-V_{th})^2 =\frac{1}{2}k(\frac{1}{\frac{1}{V_g(0)-V_s-V_{th}}-\frac{K}{C}\tau}+V_{s}-V_{dd})^2 $$
$$ i_{ds} = \frac{1}{2}K[\frac{C(V_{ref}-V_s-V_{th})}{C-K(V_{ref}-V_s-V_{th})\tau}+V_s-V_{dd}]^2 $$
$$ \frac{\partial i_{ds}}{\partial V_s} = K[\frac{C(V_{ref}-V_s-V_{th})}{C-K(V_{ref}-V_s-V_{th})\tau}+V_s-V_{dd}]\{\frac{-C[C-K(V_{ref}-V_s-V_{th})\tau]-C(V_{ref}-V_s-V_{th})K\tau}{[C-K(V_{ref}-V_s-V_{th})]^2}+1\} $$

## Introduction of $\beta$
$$ \beta = \frac{1}{\frac{V_{th}}{V_{ref}-V_s-V_{th}}-\frac{K}{C}\tau V_{th}} +2 $$
$$ V_g = \beta (V_{th}-V_s) $$
Emission stage $ V_{gs} = \beta (V_{th}-V_s) - V_{dd} $
$$i_{ds}=\frac{1}{2}k[\beta (V_{th}-V_s) - V_{dd}-V_{th}]^2 $$
$$ \frac{\partial i_{ds}}{\partial V_s}=-k\beta V_s [\beta (V_{th}-V_s) - V_{dd}-V_{th}] $$
This equation of $\frac{\partial i_{ds}}{\partial V_s}=0$ has two solutions
$$V_s = 0$$
$$V_s = \frac{(\beta-1)V_{th}-V_{dd}}{\beta} $$